add wf to local sim

theories/opt/foo.v
@@ -1,9 +1,6 @@
-From stbor.lang Require Import steps_progress steps_inversion.
-From stbor.sim Require Import local invariant.
+From stbor.sim Require Import local invariant one_step.
 
-Definition sim_body := sim_local_body wsat vrel_expr.
-Definition sim_fun := sim_local_fun wsat vrel_expr.
-Definition sim_funs := sim_local_funs wsat vrel_expr.
+Set Default Proof Using "Type".
 
 Definition foo_s : function :=
   fun: [],
@@ -38,58 +35,10 @@ Definition foo_t : function :=
   Free "y"
   .
 
-Lemma subst_l_is_Some_length xl el e e' :
-  subst_l xl el e = Some e' → length xl = length el.
-Proof.
-  revert e' el. induction xl as [|x xl IH] => e' el; [by destruct el|].
-  destruct el as [|e1 el]; [done|].
-  rewrite /= /subst'. intros Eq. f_equal.
-  destruct (subst_l xl el e) as [e2|] eqn:Eqs; [|done]. simplify_option_eq.
-  by apply (IH _ _ Eqs).
-Qed.
-
-Lemma subst_l_nil_is_Some el e e' :
-  subst_l [] el e = Some e' → e' = e.
-Proof.
-  intros Eq.
-  have EqN: el = [].
-  { apply nil_length_inv. by rewrite -(subst_l_is_Some_length _ _ _ _ Eq). }
-  subst el. simpl in Eq. by simplify_eq.
-Qed.
-
-(* Lemma sim_local_body_InitCall_aux (fns_s fns_t: fn_env) r (es et: expr) σs σt et' ct'
-  (VL: ✓ r) (WS: wsat r σs σt)
-  (ST: (InitCall et, (mkConfig fns_t σt)) ~t~> (et', ct')) :
-  let σt' := mkState σt.(shp) σt.(sst) (σt.(snc) :: σt.(scs)) σt.(snp) (S σt.(snc)) in
-  let σs' := mkState σs.(shp) σs.(sst) (σs.(snc) :: σs.(scs)) σs.(snp) (S σs.(snc)) in
-  et' = et ∧ ct' = mkConfig fns_t σt' ∧
-  (InitCall es, (mkConfig fns_s σs)) ~t~>* (es, mkConfig fns_s σs').
-Proof.
-Abort. *)
-
-From iris.algebra Require Import updates local_updates.
-
-Lemma sim_body_InitCall fns fnt r n es et σs σt :
-  let σs' := mkState σs.(shp) σs.(sst) (σs.(snc) :: σs.(scs)) σs.(snp) (S σs.(snc)) in
-  let σt' := mkState σt.(shp) σt.(sst) (σt.(snc) :: σt.(scs)) σt.(snp) (S σt.(snc)) in
-  let r'  : resUR := (∅, {[σt.(snc) := to_callStateR (csOwned ∅)]}) in
-  sim_body fns fnt (r ⋅ r') n (EndCall es) σs' (EndCall et) σt' →
-  sim_body fns fnt r n (InitCall es) σs (InitCall et) σt.
-Proof.
-  intros σs' σt' r' SIM. pfold. apply sim_local_body_step.
-  intros. exists (EndCall es), σs', (r ⋅ r').
-  destruct (tstep_init_call_inv _ _ _ _ _ STEPT).
-  subst e_tgt' σ_tgt'.
-  exists n. split; last split; last split.
-  - left. apply tc_once. by eapply (head_step_tstep _ []), initcall_head_step.
-  - rewrite cmra_assoc. admit.
-  - rewrite cmra_assoc. admit.
-  - by punfold SIM.
-Admitted.
-
 Lemma foo_sim_fun fns fnt : sim_fun fns fnt foo_s foo_t.
 Proof.
-  move => r es et els elt σs σt _ _ _ /subst_l_nil_is_Some ? /subst_l_nil_is_Some ?.
+  move => r es et els elt σs σt _ _ _
+          /subst_l_nil_is_Some ? /subst_l_nil_is_Some ?.
   subst es et. clear els elt.
 
   (* InitCall *)
