theories/sim/local.v
@@ -25,6 +25,8 @@ Inductive _sim_local_body
       (VALID: ✓ (r_f ⋅ r))
       (* and has world satisfaction *)
       (WSAT: wsat (r_f ⋅ r) σ_src σ_tgt)
+      (* both states are wellformed *)
+      (WFS: Wf σ_src) (WFT: Wf σ_tgt)
       (* if tgt can locally make 1 step *)
       (STEPT: (e_tgt, σ_tgt) ~{fnt}~> (e_tgt', σ_tgt')),
       (* then we locally can makes some step and pick a new resource r' *)
@@ -32,6 +34,7 @@ Inductive _sim_local_body
         ((e_src, σ_src) ~{fns}~>+ (e_src', σ_src') ∨
          ((idx' < idx)%nat ∧ (e_src', σ_src') = (e_src, σ_src))) ∧
         ✓ (r_f ⋅ r') ∧ wsat (r_f ⋅ r') σ_src' σ_tgt' ∧
+        Wf σ_src' ∧ Wf σ_tgt' ∧
         sim_local_body r' idx' e_src' σ_src' e_tgt' σ_tgt')
     : _sim_local_body sim_local_body r idx e_src σ_src e_tgt σ_tgt
 (* If tgt prepares to make a call to [name], src should be able to make the same
@@ -46,6 +49,8 @@ Inductive _sim_local_body
         (VALID: ✓ (r_f ⋅ r))
         (* and has world satisfaction *)
         (WSAT : wsat (r_f ⋅ r) σ_src σ_tgt)
+        (* both states are wellformed *)
+        (WFS: Wf σ_src) (WFT: Wf σ_tgt)
         (* tgt is ready to make a call of [name] *)
         (VTGT : Forall (λ ei, is_Some (to_value ei)) el_tgt),
         (* then src is also ready to make a call of [name] *)
@@ -63,6 +68,8 @@ Inductive _sim_local_body
              our local resource r and have world satisfaction *)
           (VALID': ✓ (r_f' ⋅ (rc ⋅ r')))
           (WSAT' : wsat (r_f ⋅ (rc ⋅ r')) σ_src' σ_tgt')
+          (* both state are wellformed *)
+          (WFS: Wf σ_src') (WFT: Wf σ_tgt')
           (* and the returned values are related w.r.t. (r ⋅ r' ⋅ r_f) *)
           (VRET  : vrel r' (Val v_src) (Val v_tgt)),
           ∃ idx', sim_local_body (rc ⋅ r') idx'
@@ -76,6 +83,7 @@ Inductive _sim_local_body
     (END: ∀ r_f eσ_tgt'
         (VALID: ✓ (r_f ⋅ r))
         (WSAT : wsat (r_f ⋅ r) σ_src σ_tgt)
+        (WFS: Wf σ_src) (WFT: Wf σ_tgt)
         (* if tgt can end call *)
         (ETGT: (EndCall (Val v_tgt), σ_tgt) ~{fnt}~> eσ_tgt'),
         (* then src can also end call *)
@@ -83,6 +91,7 @@ Inductive _sim_local_body
         (EndCall (Val v_src), σ_src) ~{fns}~> eσ_src' ∧
         (* and re-establish wsat *)
         ✓ (r_f ⋅ r') ∧ wsat (r_f ⋅ r') eσ_src'.2 eσ_tgt'.2 ∧
+        Wf eσ_src'.2 ∧ Wf eσ_tgt'.2 ∧
         (* and the returned values are related *)
         vrel r' (Val v_src) (Val v_tgt))
     : _sim_local_body sim_local_body r idx e_src σ_src e_tgt σ_tgt
@@ -98,45 +107,6 @@ Proof.
 Qed.
 
 Definition sim_local_body := paco6 _sim_local_body bot6.
-
-Lemma sim_local_body_resource_mono r1 r2
-  (SAT_DOWNWARD: ∀ r1 r2, r1 ≼ r2 → wsat r2 <2= wsat r1) :
-  r1 ≼ r2 → sim_local_body r1 <5= sim_local_body r2.
-Proof.
-  revert r1 r2. pcofix CIH. intros r1 r2 LE idx es σs et σt SIM.
-  pfold. punfold SIM; [|apply sim_local_body_mono].
-  inversion SIM; subst.
-  - by eapply sim_local_body_stuck.
-  - eapply sim_local_body_step.
-    intros r_f et' ct' VL2 WS2 STEPT.
-    have VL1: ✓ (r_f ⋅ r1).
-    { eapply cmra_valid_included; [exact VL2|by apply cmra_mono_l]. }
-    have WS1: wsat (r_f ⋅ r1) σs σt.
-    { eapply SAT_DOWNWARD; [by apply cmra_mono_l|exact WS2]. }
-    destruct (STEP _ _ _ VL1 WS1 STEPT) as
-      (es' & cs' & r' & idx' & STEPS' & VL' & WS' & SIM').
-    exists es', cs', r', idx'. do 3 (split; [done|]).
-    right. eapply CIH; eauto. by inversion SIM'.
-  - eapply sim_local_body_step_over_call; eauto.
-    intros r_f VL2 WS2 FAT.
-    have VL1: ✓ (r_f ⋅ r1).
-    { eapply cmra_valid_included; [exact VL2|by apply cmra_mono_l]. }
-    have WS1: wsat (r_f ⋅ r1) σs σt.
-    { eapply SAT_DOWNWARD; [by apply cmra_mono_l|exact WS2]. }
-    destruct (STEPOVER _ VL1 WS1 FAT)
-      as (es' & cs & rc & rv & STEPS & FAS & VL & WS & VREL & HK).
-    exists es', cs, rc, rv. do 5 (split; [done|]).
-    intros r_f' r' vs vt cs' ct' VL' WS' VREL'.
-    destruct (HK _ _ _ _ _ _ VL' WS' VREL') as [idx' HK2].
-    exists idx'. right. eapply CIH; [eauto|by inversion HK2].
-  - eapply sim_local_body_end_call; [eauto..|].
-    intros r_f ct' VL2 WS2 STEPT.
-    have VL1: ✓ (r_f ⋅ r1).
-    { eapply cmra_valid_included; [exact VL2|by apply cmra_mono_l]. }
-    have WS1: wsat (r_f ⋅ r1) σs σt.
-    { eapply SAT_DOWNWARD; [by apply cmra_mono_l|exact WS2]. }
-    naive_solver.
-Qed.
 
 (* Simulating functions: assuming the calls have been initialized. *)
 Definition sim_local_fun (fn_src fn_tgt : function) : Prop :=
