theories/sim/one_step.v
@@ -1,0 +1,51 @@
+From iris.algebra Require Import local_updates.
+
+From stbor.lang Require Import steps_progress steps_inversion.
+From stbor.sim Require Import local invariant.
+
+Set Default Proof Using "Type".
+
+Lemma local_update_discrete_valid_frame `{CmraDiscrete A} (r_f r r' : A) :
+  ✓ (r_f ⋅ r) → (r_f ⋅ r, r) ~l~> (r_f ⋅ r', r') → ✓ (r_f ⋅ r').
+Proof.
+  intros VALID UPD. apply cmra_discrete_valid.
+  apply (UPD O (Some r_f)); [by apply cmra_discrete_valid_iff|by rewrite /= comm].
+Qed.
+
+Notation sim_body := (sim_local_body wsat vrel_expr).
+Notation sim_fun := (sim_local_fun wsat vrel_expr).
+Notation sim_funs := (sim_local_funs wsat vrel_expr).
+
+Lemma sim_body_InitCall fns fnt r n es et σs σt :
+  let σs' := mkState σs.(shp) σs.(sst) (σs.(snc) :: σs.(scs)) σs.(snp) (S σs.(snc)) in
+  let σt' := mkState σt.(shp) σt.(sst) (σt.(snc) :: σt.(scs)) σt.(snp) (S σt.(snc)) in
+  let r'  : resUR := (∅, {[σt.(snc) := to_callStateR (csOwned ∅)]}) in
+  sim_body fns fnt (r ⋅ r') n (EndCall es) σs' (EndCall et) σt' →
+  sim_body fns fnt r n (InitCall es) σs (InitCall et) σt.
+Proof.
+  intros σs' σt' r' SIM. pfold. apply sim_local_body_step.
+  intros. exists (EndCall es), σs', (r ⋅ r').
+  destruct (tstep_init_call_inv _ _ _ _ _ STEPT).
+  subst e_tgt' σ_tgt'.
+  have STEPS: (InitCall es, σs) ~{fns}~> (EndCall es, σs').
+  { by eapply (head_step_tstep _ []), initcall_head_step. }
+  have FRESH: (r_f ⋅ r).2 !! σt.(snc) = None.
+  { destruct ((r_f ⋅ r).2 !! σt.(snc)) as [cs|] eqn:Eqcs; [|done].
+    exfalso. destruct WSAT as [WF _].
+    by apply (lt_irrefl σt.(snc)), WF, (elem_of_dom_2 _ _ _ Eqcs). }
+  have LOCAL: (r_f ⋅ r ⋅ ε, ε) ~l~> (r_f ⋅ r ⋅ r', r').
+  { apply prod_local_update_2.
+    rewrite /= right_id  (comm _ (_ ⋅ _)) -insert_singleton_op //.
+    by apply alloc_singleton_local_update. }
+  exists n. split; last split; last split; last split; last split; cycle 3.
+  { (* WF src *)    by apply (tstep_wf _ _ _ STEPS WFS). }
+  { (* WF tgt *)    by apply (tstep_wf _ _ _ STEPT WFT). }
+  { (* sim cont *)  by punfold SIM. }
+  { (* STEP src *)  left. by apply tc_once. }
+  { (* VALID new *)
+    rewrite assoc.
+    apply (local_update_discrete_valid_frame (r_f ⋅ r) ε r'); [|done].
+    by rewrite right_id. }
+  (* WSAT new *)
+
+Admitted.
